workspace/src/login/DY.Login.Invariants.fst
@@ -29,6 +29,7 @@ let aead_predicates_login: list (string & aead_crypto_predicate) = [
   aead_crypto_predicate_and_tag_communication_layer_reqres (http_t web_types kv_types);
 ]
 
+[@@ "opaque_to_smt"]
 let crypto_predicates_login: crypto_predicates = {
   default_crypto_predicates with
   pke_pred = mk_pke_predicate pke_predicates_login;
@@ -41,13 +42,33 @@ instance crypto_invariants_login: crypto_invariants = {
   preds = crypto_predicates_login;
 }
 
+#push-options "--fuel 2 --ifuel 0"
+let _ = (
+  reveal_opaque (`%crypto_predicates_login) crypto_predicates_login;
+  assert_norm(List.Tot.no_repeats_p (List.Tot.map fst (pke_predicates_login)));
+  do_split_boilerplate mk_pke_predicate_correct pke_predicates_login
+)
+let _ = (
+  reveal_opaque (`%crypto_predicates_login) crypto_predicates_login;
+  assert_norm(List.Tot.no_repeats_p (List.Tot.map fst (sign_predicates_login)));
+  do_split_boilerplate mk_sign_predicate_correct sign_predicates_login
+)
+let _ = (
+  reveal_opaque (`%crypto_predicates_login) crypto_predicates_login;
+  do_split_boilerplate mk_aead_predicate_correct aead_predicates_login
+)
+#pop-options
+
 (*** HTTP predicates ***)
 
 val wt_send_request_pred_key_username: wt_send_request_pred_key "username"
 let wt_send_request_pred_key_username = {
   pred = (fun tr client server key_label http_req -> (
     match get_principal_from_json_encoded "username" http_req.body with
-    | Some username -> username == client
+    | Some username -> (
+      username == client /\
+      event_triggered tr client (ClientAuthenticatesToServer client server)
+    )
     | None -> False
   ));
   pred_later = (fun tr1 tr2 client server key_label http_req -> ());
@@ -56,11 +77,7 @@ let wt_send_request_pred_key_username = {
 #push-options "--ifuel 1"
 val wt_send_request_pred_key_password: wt_send_request_pred_key "password"
 let wt_send_request_pred_key_password = {
-  pred = (fun tr client server key_label http_req ->
-    match get_bytes_from_json_encoded "password" http_req.body with
-    | Some password -> is_secret (comm_label client server) tr password
-    | None -> False
-  );
+  pred = (fun tr client server key_label http_req -> True);
   pred_later = (fun tr1 tr2 client server key_label http_req -> ());
 }
 #pop-options
@@ -113,12 +130,16 @@ instance browser_predicates_login: browser_preds web_types kv_types = {
 
 (*** Event invariant ***)
 
+#push-options "--ifuel 1"
 let event_predicate_login: event_predicate event_t =
   fun tr prin e ->
     match e with
-    | ServerAuthenticatedUser client server request key ->
+    | ClientAuthenticatesToServer client server -> True
+    | ServerAuthenticatedClient client server ->
       prin == server /\
-      event_triggered tr client (CommClientSendRequest Unauthenticated client server (Request request) key <: communication_reqres_event (http_t web_types kv_types))
+      (event_triggered tr client (ClientAuthenticatesToServer client server) \/
+       is_corrupt tr (principal_label client) \/ is_corrupt tr (principal_label server))
+#pop-options
 
 (*** Protocol state invariant ***)
 
@@ -127,6 +148,7 @@ let state_predicate_login: local_state_predicate state_t = {
   pred = (fun tr prin sess_id st ->
     match st with
     | InitialState client server password ->
+      // TODO remove one principal
       (prin == client \/ prin == server) /\
       is_secret (comm_label client server) tr password
     | SendRequest hmeta_data ->
@@ -166,6 +188,7 @@ let all_events_login: list (string & compiled_event_predicate) =
     (event_predicate_communication_layer_reqres_and_tag (http_t web_types kv_types))
     [mk_event_tag_and_pred event_predicate_login]
 
+[@@ "opaque_to_smt"]
 let trace_invariants_login: trace_invariants = {
   state_pred = mk_state_pred all_sessions_login;
   state_update_pred = mk_state_update_pred all_session_updates_login;
@@ -197,9 +220,7 @@ let _ = (
   assert_norm(List.Tot.no_repeats_p (List.Tot.map fst (all_events_login)));
   do_split_boilerplate mk_event_pred_correct all_events_login
 )
-(*let _ = do_split_boilerplate mk_pke_predicate_correct pke_predicates_login
-let _ = do_split_boilerplate mk_sign_predicate_correct sign_predicates_login
-let _ = do_split_boilerplate mk_aead_predicate_correct aead_predicates_login*)
+
 let _ = do_split_boilerplate mk_wt_send_request_pred_correct request_predicates_login
 let _ = do_split_boilerplate mk_wt_send_response_pred_correct response_predicates_login
 
@@ -208,157 +229,8 @@ let _:squash (has_private_keys_invariant /\ has_private_keys_state_update_invari
 let _:squash (has_local_state_predicate state_predicate_login) = reveal_opaque (`%trace_invariants_login) trace_invariants_login
 let _:squash (has_local_state_update_predicate state_update_predicate_login) = reveal_opaque (`%trace_invariants_login) trace_invariants_login
 let _:squash (has_event_pred event_predicate_login) = reveal_opaque (`%trace_invariants_login) trace_invariants_login
+let _:squash (has_communication_layer_reqres_predicates (http_t web_types kv_types)) = reveal_opaque (`%crypto_predicates_login) crypto_predicates_login; reveal_opaque (`%trace_invariants_login) trace_invariants_login
 
 let _:squash (has_web_types_request_key_pred (|"username", wt_send_request_pred_key_username|)) = reveal_opaque (`%trace_invariants_login) trace_invariants_login
 let _:squash (has_web_types_request_key_pred (|"password", wt_send_request_pred_key_password|)) = reveal_opaque (`%trace_invariants_login) trace_invariants_login
 #pop-options
-
-(*)
-val login_state_predicates_correct:
-  squash (for_allP has_local_bytes_state_predicate all_sessions_login)
-let login_state_predicates_correct =
-  assert_norm (List.Tot.no_repeats_p (List.Tot.map dfst all_sessions_login));
-  mk_state_pred_correct all_sessions_login
-
-val login_state_update_predicates_correct:
-  squash (for_allP has_local_bytes_state_update_predicate all_session_updates_login)
-let login_state_update_predicates_correct =
-  assert_norm (List.Tot.no_repeats_p (List.Tot.map dfst all_session_updates_login));
-  mk_state_update_pred_correct all_session_updates_login
-
-val login_event_predicates_correct:
-  squash (for_allP has_compiled_event_pred all_events_login)
-let login_event_predicates_correct =
-  assert_norm (List.Tot.no_repeats_p (List.Tot.map fst all_events_login));
-  mk_event_pred_correct all_events_login
-
-val login_has_pke_predicate:
-  squash (
-    has_pke_predicate
-      (pke_crypto_predicate_and_tag_communication_layer_reqres
-        (http_t web_types kv_types))
-  )
-let login_has_pke_predicate = ()
-
-val login_has_sign_predicate:
-  squash (
-    has_sign_predicate
-      (sign_crypto_predicate_and_tag_communication_layer_reqres
-        (http_t web_types kv_types))
-  )
-let login_has_sign_predicate = ()
-
-val login_has_aead_predicate:
-  squash (
-    has_aead_predicate
-      (aead_crypto_predicate_and_tag_communication_layer_reqres
-        (http_t web_types kv_types))
-  )
-let login_has_aead_predicate = ()
-
-#push-options "--ifuel 1 --z3rlimit 100"
-val login_has_state_predicate:
-  squash (has_local_state_predicate state_predicate_login)
-let login_has_state_predicate =
-  login_state_predicates_correct;
-  for_allP_eq has_local_bytes_state_predicate all_sessions_login;
-  assert_norm (
-    memP (mk_local_state_tag_and_pred state_predicate_login) all_sessions_login
-  );
-  ()
-
-val login_has_state_update_predicate:
-  squash (has_local_state_update_predicate state_update_predicate_login)
-let login_has_state_update_predicate =
-  login_state_update_predicates_correct;
-  for_allP_eq has_local_bytes_state_update_predicate all_session_updates_login;
-  assert_norm (
-    memP
-      (mk_local_state_tag_and_update_pred state_update_predicate_login)
-      all_session_updates_login
-  );
-  ()
-
-val login_has_event_predicate:
-  squash (has_event_pred event_predicate_login)
-let login_has_event_predicate =
-  login_event_predicates_correct;
-  for_allP_eq has_compiled_event_pred all_events_login;
-  assert_norm (memP (mk_event_tag_and_pred event_predicate_login) all_events_login);
-  ()
-
-val login_has_pki_predicates:
-  squash (has_pki_invariant /\ has_pki_state_update_invariant)
-let login_has_pki_predicates =
-  login_state_predicates_correct;
-  for_allP_eq has_local_bytes_state_predicate all_sessions_login;
-  assert_norm (memP pki_tag_and_invariant all_sessions_login);
-  login_state_update_predicates_correct;
-  for_allP_eq has_local_bytes_state_update_predicate all_session_updates_login;
-  assert_norm (memP pki_tag_and_state_update_pred all_session_updates_login);
-  ()
-
-val login_has_private_key_predicates:
-  squash (has_private_keys_invariant /\ has_private_keys_state_update_invariant)
-let login_has_private_key_predicates =
-  login_state_predicates_correct;
-  for_allP_eq has_local_bytes_state_predicate all_sessions_login;
-  assert_norm (memP private_keys_tag_and_invariant all_sessions_login);
-  login_state_update_predicates_correct;
-  for_allP_eq has_local_bytes_state_update_predicate all_session_updates_login;
-  assert_norm (
-    memP private_keys_tag_and_state_update_pred all_session_updates_login
-  );
-  ()
-
-val login_has_username_request_predicate:
-  squash (
-    has_web_types_request_key_pred
-      (|"username", wt_send_request_pred_key_username|)
-  )
-let login_has_username_request_predicate = ()
-
-val login_has_wt_send_request_pred_key_password:
-  squash (
-    has_web_types_request_key_pred
-      (|"password", wt_send_request_pred_key_password|)
-  )
-let login_has_wt_send_request_pred_key_password = ()
-
-val login_has_id_response_predicate:
-  squash (
-    has_web_types_response_key_pred
-      (|"id", wt_send_request_pred_key_true "id"|)
-  )
-let login_has_id_response_predicate = ()
-
-val login_has_username_response_predicate:
-  squash (
-    has_web_types_response_key_pred
-      (|"username", wt_send_request_pred_key_true "username"|)
-  )
-let login_has_username_response_predicate = ()
-
-val login_has_email_response_predicate:
-  squash (
-    has_web_types_response_key_pred
-      (|"email", wt_send_request_pred_key_true "email"|)
-  )
-let login_has_email_response_predicate = ()
-
-val login_has_first_name_response_predicate:
-  squash (
-    has_web_types_response_key_pred
-      (|"firstName", wt_send_request_pred_key_true "firstName"|)
-  )
-let login_has_first_name_response_predicate = ()
-
-val login_has_last_name_response_predicate:
-  squash (
-    has_web_types_response_key_pred
-      (|"lastName", wt_send_request_pred_key_true "lastName"|)
-  )
-let login_has_last_name_response_predicate = ()
-
-#pop-options
-*)
