workspace/src/login/DY.Login.SecurityProperties.fst
@@ -1,0 +1,44 @@
+module DY.Login.SecurityProperties
+
+open Comparse
+open FStar.List.Tot { for_allP }
+open DY.Core
+open DY.Lib
+
+open DY.Lib.Web
+open DY.Lib.Web.HTTP.Invariants
+open DY.Lib.Web.Data.Default.Invariants
+
+open DY.Login.Protocol
+open DY.Login.Invariants
+
+#set-options "--fuel 0 --ifuel 0 --z3cliopt 'smt.qi.eager_threshold=100'"
+
+val user_authentication:
+  tr:trace -> client:principal -> server:principal -> 
+  Lemma
+  (requires
+    trace_invariant tr /\
+    event_triggered tr server (ServerAuthenticatedClient client server)
+  )
+  (ensures (
+    event_triggered tr client (ClientAuthenticatesToServer client server) \/
+    is_corrupt tr (principal_label client) \/ is_corrupt tr (principal_label server)
+  ))
+let user_authentication tr client server = ()
+
+val password_secrecy:
+  tr:trace -> client:principal -> server:principal -> password:bytes ->
+  Lemma
+  (requires
+    trace_invariant tr /\
+    attacker_knows tr password /\ (
+      (exists sess_id. state_was_set tr client sess_id (InitialState client server password)) \/
+      (exists sess_id. state_was_set tr server sess_id (InitialState client server password))
+    )
+  )
+  (ensures
+    is_corrupt tr (principal_label client) \/ is_corrupt tr (principal_label server)
+  )
+let password_secrecy tr client server password =
+  attacker_only_knows_publishable_values tr password
